Reformat code according to Dafny style guide
Mostly indentation changes.
Capitalize method names.

src/SDK/MessageHeader/Definitions.dfy
@@ -3,41 +3,40 @@ include "../../StandardLibrary/StandardLibrary.dfy"
 include "../Materials.dfy"
 
 module MessageHeader.Definitions {
-    import AlgorithmSuite
-    import opened StandardLibrary
-    import opened UInt = StandardLibrary.UInt
-    import Materials
+  import AlgorithmSuite
+  import opened StandardLibrary
+  import opened UInt = StandardLibrary.UInt
+  import Materials
 
-    /*
-    * Header body type definition
-    */
-    type T_Version         = x | x == 0x01 /*Version 1.0*/ witness 0x01
-    type T_Type            = x | x == 0x80 /*Customer Authenticated Encrypted Data*/ witness 0x80
-    type T_MessageID       = x: seq<uint8> | |x| == 16 witness [0,0,0,0,0,0,0,0,0,0,0,0,0,0,0,0]
-    type T_Reserved        = x: seq<uint8> | x == [0,0,0,0] witness [0,0,0,0]
-    datatype T_ContentType = NonFramed | Framed
-    type EncCtx            = Materials.EncryptionContext
-    datatype T_AAD         = AAD(kvPairs: EncCtx) | EmptyAAD
+  /*
+  * Header body type definition
+  */
+  type T_Version               = x | x == 0x01 /*Version 1.0*/ witness 0x01
+  type T_Type                  = x | x == 0x80 /*Customer Authenticated Encrypted Data*/ witness 0x80
+  type T_MessageID             = x: seq<uint8> | |x| == 16 witness [0,0,0,0,0,0,0,0,0,0,0,0,0,0,0,0]
+  type T_Reserved              = x: seq<uint8> | x == [0,0,0,0] witness [0,0,0,0]
+  datatype T_ContentType       = NonFramed | Framed
+  type EncCtx                  = Materials.EncryptionContext
+  datatype T_AAD               = AAD(kvPairs: EncCtx) | EmptyAAD
 
-    type EDKEntry          = Materials.EncryptedDataKey
-    datatype T_EncryptedDataKeys
-                           = EncryptedDataKeys(entries: seq<EDKEntry>)
+  type EDKEntry                = Materials.EncryptedDataKey
+  datatype T_EncryptedDataKeys = EncryptedDataKeys(entries: seq<EDKEntry>)
 
-    datatype HeaderBody    = HeaderBody(
-                                version: T_Version,
-                                typ: T_Type,
-                                algorithmSuiteID: AlgorithmSuite.ID,
-                                messageID: T_MessageID,
-                                aad: T_AAD,
-                                encryptedDataKeys: T_EncryptedDataKeys,
-                                contentType: T_ContentType,
-                                reserved: T_Reserved,
-                                ivLength: uint8,
-                                frameLength: uint32)
+  datatype HeaderBody          = HeaderBody(
+                                   version: T_Version,
+                                   typ: T_Type,
+                                   algorithmSuiteID: AlgorithmSuite.ID,
+                                   messageID: T_MessageID,
+                                   aad: T_AAD,
+                                   encryptedDataKeys: T_EncryptedDataKeys,
+                                   contentType: T_ContentType,
+                                   reserved: T_Reserved,
+                                   ivLength: uint8,
+                                   frameLength: uint32)
 
-    /*
-    * Header authentication type definition
-    */
+  /*
+  * Header authentication type definition
+  */
 
-    datatype HeaderAuthentication = HeaderAuthentication(iv: array<uint8>, authenticationTag: array<uint8>)
+  datatype HeaderAuthentication = HeaderAuthentication(iv: array<uint8>, authenticationTag: array<uint8>)
 }
