src/SDK/MessageHeader/MessageHeader.dfy
@@ -8,70 +8,65 @@ include "../../Util/Streams.dfy"
 include "../../StandardLibrary/StandardLibrary.dfy"
 
 module MessageHeader {
-    import AlgorithmSuite
-    import opened StandardLibrary
-    import opened Streams
+  import AlgorithmSuite
+  import opened StandardLibrary
+  import Streams
 
-    /*
-     * Definition of the message header, i.e., the header body and the header authentication
-     */
-    class Header {
-        var body: Option<Definitions.HeaderBody>
-        var auth: Option<Definitions.HeaderAuthentication>
+  import D = Deserialize
+  import S = Serialize
 
-        constructor () {
-            body := None;
-            auth := None;
-        }
+  /*
+   * Definition of the message header, i.e., the header body and the header authentication
+   */
+  class Header {
+    var body: Option<Definitions.HeaderBody>
+    var auth: Option<Definitions.HeaderAuthentication>
 
-        method deserializeHeader(is: StringReader)
-            requires is.Valid()
-            modifies is, `body, `auth
-            requires body.None? || auth.None?
-            ensures body.Some? && auth.Some? ==> Validity.ValidHeaderBody(body.get)
-            ensures body.Some? && auth.Some? ==> Validity.ValidHeaderAuthentication(auth.get, body.get.algorithmSuiteID)
-            // TODO: is this the right decision?
-            ensures body.Some? <==> auth.Some?
-            ensures body.None? <==> auth.None? // redundant
-            ensures is.Valid()
-        {
-            {
-                var res := Deserialize.headerBody(is);
-                match res {
-                    case Success(body_) =>
-                        // How does Dafny know the following assertion holds with Validity.ValidHeaderBody being opaque?
-                        assert body_.algorithmSuiteID in AlgorithmSuite.Suite.Keys; // nfv
-                        var res := Deserialize.headerAuthentication(is, body_);
-                        match res {
-                            case Success(auth_) =>
-                                body := Some(body_);
-                                auth := Some(auth_);
-                                assert Validity.ValidHeaderBody(body.get);
-                            case Failure(e)    => {
-                                print "Could not deserialize message header: " + e + "\n";
-                                body := None;
-                                auth := None;
-                                return;
-                            }
-                        }
-                    case Failure(e)    => {
-                        print "Could not deserialize message header: " + e + "\n";
-                        body := None;
-                        auth := None;
-                        return;
-                    }
-                }
-            }
-        }
-
-        method serializeHeader(os: StringWriter) returns (ret: Result<nat>)
-            requires os.Valid()
-            requires body.Some?
-            requires Validity.ValidHeaderBody(body.get)
-            modifies os.Repr
-            ensures os.Valid()
-        {
-            ret := Serialize.headerBody(os, body.get);
-        }
+    constructor () {
+      body, auth := None, None;
     }
+
+    method Deserialize(is: Streams.StringReader)
+      requires is.Valid()
+      requires body.None? || auth.None?
+      modifies is, `body, `auth
+      ensures body.Some? && auth.Some? ==> Validity.ValidHeaderBody(body.get)
+      ensures body.Some? && auth.Some? ==> Validity.ValidHeaderAuthentication(auth.get, body.get.algorithmSuiteID)
+      // TODO: is this the right decision?
+      ensures body.Some? <==> auth.Some?
+      ensures body.None? <==> auth.None? // redundant
+      ensures is.Valid()
+    {
+      var res := D.DeserializeHeaderBody(is);
+      match res {
+        case Success(body_) =>
+          // How does Dafny know the following assertion holds with Validity.ValidHeaderBody being opaque?
+          assert body_.algorithmSuiteID in AlgorithmSuite.Suite.Keys; // nfv
+          var res := D.DeserializeAuthenticationHeader(is, body_);
+          match res {
+            case Success(auth_) =>
+              body, auth := Some(body_), Some(auth_);
+              assert Validity.ValidHeaderBody(body.get);
+            case Failure(e) =>
+              print "Could not deserialize message header: " + e + "\n";
+              body, auth := None, None;
+              return;
+          }
+        case Failure(e) =>
+          print "Could not deserialize message header: " + e + "\n";
+          body, auth := None, None;
+          return;
+      }
+    }
+
+    method Serialize(os: Streams.StringWriter) returns (ret: Result<nat>)
+      requires os.Valid()
+      requires body.Some?
+      requires Validity.ValidHeaderBody(body.get)
+      modifies os.Repr
+      ensures os.Valid()
+    {
+      ret := S.SerializeHeaderBody(os, body.get);
+    }
+  }
 }
