src/SDK/MessageHeader/Serialize.dfy
@@ -11,168 +11,159 @@ include "../../Util/Streams.dfy"
 include "../../StandardLibrary/StandardLibrary.dfy"
 
 module MessageHeader.Serialize {
-    import opened Definitions
-    import opened SerializeAAD
-    import opened SerializeEDK
-    import opened Validity
+  import opened Definitions
+  import SerializeAAD
+  import SerializeEDK
+  import opened Validity
 
-    import opened Streams
-    import opened StandardLibrary
-    import opened UInt = StandardLibrary.UInt
+  import Streams
+  import opened StandardLibrary
+  import opened UInt = StandardLibrary.UInt
 
-    lemma {:axiom} Assume(b : bool) ensures b
+  lemma {:axiom} Assume(b: bool)
+    ensures b
 
-    function {:opaque} serialize(hb: HeaderBody): seq<uint8>
-        requires ValidHeaderBody(hb)
+  function {:opaque} Serialize(hb: HeaderBody): seq<uint8>
+    requires ValidHeaderBody(hb)
+  {
+    reveal ValidHeaderBody();
+    [hb.version as uint8] +
+    [hb.typ as uint8] +
+    UInt16ToSeq(hb.algorithmSuiteID as uint16) +
+    hb.messageID +
+    SerializeAAD.SerializeAAD(hb.aad) +
+    SerializeEDK.SerializeEDK(hb.encryptedDataKeys) +
+    (match hb.contentType case NonFramed => [0x01] case Framed => [0x02]) +
+    hb.reserved +
+    [hb.ivLength] +
+    UInt32ToSeq(hb.frameLength)
+  }
+
+  method SerializeHeaderBody(os: Streams.StringWriter, hb: HeaderBody) returns (ret: Result<nat>)
+    requires os.Valid() && ValidHeaderBody(hb)
+    modifies os`data
+    // It's crucial to require no aliasing here
+    ensures os.Valid() && ValidHeaderBody(hb)
+    // TODO: these should probably be enabled
+    //ensures old(|os.data|) <= |os.data|
+    ensures match ret
+      case Success(totalWritten) =>
+        var serHb := (reveal Serialize(); Serialize(hb));
+        var initLen := old(|os.data|);
+        && totalWritten == |serHb|
+        && initLen+totalWritten == |os.data|
+        && serHb[..totalWritten] == os.data[initLen..initLen+totalWritten]
+      case Failure(e) => true
+  {
+    var totalWritten := 0;
+    ghost var initLen := |os.data|;
+    reveal ValidHeaderBody();
+    reveal ValidAAD();
+    reveal ValidEncryptedDataKeys();
     {
-        reveal ValidHeaderBody();
-        [hb.version as uint8] +
-        [hb.typ as uint8] +
-        UInt16ToSeq(hb.algorithmSuiteID as uint16) +
-        hb.messageID +
-        serializeAAD(hb.aad) +
-        serializeEDK(hb.encryptedDataKeys) +
-        (match hb.contentType case NonFramed => [0x01] case Framed => [0x02]) +
-        hb.reserved +
-        [hb.ivLength] +
-        UInt32ToSeq(hb.frameLength)
+      ret := os.WriteSingleByteSimple(hb.version as uint8);
+      match ret {
+        case Success(len) => totalWritten := totalWritten + len;
+        case Failure(e)  =>
+          return ret;
+      }
     }
 
-    method headerBody(os: StringWriter, hb: HeaderBody) returns (ret: Result<nat>)
-        requires os.Valid()
-        modifies os`data
-        requires ValidHeaderBody(hb)
-        // It's crucial to require no aliasing here
-        ensures os.Valid()
-        // TODO: these should probably be enabled
-        //ensures unchanged(os`Repr)
-        //ensures unchanged(ReprEncryptedDataKeys(hb.encryptedDataKeys))
-        //ensures old(|os.data|) <= |os.data|
-        ensures ValidHeaderBody(hb)
-        ensures
-            match ret
-                case Success(totalWritten) =>
-                    var serHb := (reveal serialize(); serialize(hb));
-                    var initLen := old(|os.data|);
-                    && totalWritten == |serHb|
-                    && initLen+totalWritten == |os.data|
-                    && serHb[..totalWritten] == os.data[initLen..initLen+totalWritten]
-                case Failure(e) => true
     {
-        var totalWritten := 0;
-        ghost var initLen := |os.data|;
-        reveal ValidHeaderBody();
-        reveal ValidAAD();
-        reveal ValidEncryptedDataKeys();
-        {
-            ret := os.WriteSingleByteSimple(hb.version as uint8);
-            match ret {
-                case Success(len) => totalWritten := totalWritten + len;
-                case Failure(e)  => {
-                    return ret;
-                }
-            }
-        }
-
-        {
-            ret := os.WriteSingleByteSimple(hb.typ as uint8);
-            match ret {
-                case Success(len) => totalWritten := totalWritten + len;
-                case Failure(e)  => {
-                    return ret;
-                }
-            }
-        }
-
-        {
-            var bytes := UInt16ToArray(hb.algorithmSuiteID as uint16);
-            ret := os.WriteSimple(bytes);
-            match ret {
-                case Success(len) => totalWritten := totalWritten + len;
-                case Failure(e)  => {
-                    return ret;
-                }
-            }
-        }
-
-        {
-            ret := os.WriteSimpleSeq(hb.messageID);
-            match ret {
-                case Success(len) => totalWritten := totalWritten + len;
-                case Failure(e)  => {
-                    return ret;
-                }
-            }
-        }
-
-        {
-            ret := serializeAADImpl(os, hb.aad);
-            match ret {
-                case Success(len) => totalWritten := totalWritten + len;
-                case Failure(e)  => {
-                    return ret;
-                }
-            }
-        }
-
-        {
-            ret := serializeEDKImpl(os, hb.encryptedDataKeys);
-            match ret {
-                case Success(len) => totalWritten := totalWritten + len;
-                case Failure(e)  => return ret;
-            }
-        }
-
-        {
-            var contentType: uint8;
-            match hb.contentType {
-                case NonFramed => contentType := 0x01;
-                case Framed    => contentType := 0x02;
-            }
-            ret := os.WriteSingleByteSimple(contentType);
-            match ret {
-                case Success(len) =>
-                    totalWritten := totalWritten + len;
-                case Failure(e)  =>
-                    return ret;
-            }
-        }
-
-        {
-            ret := os.WriteSimpleSeq(hb.reserved);
-            match ret {
-                case Success(len) => totalWritten := totalWritten + len;
-                case Failure(e)  => return ret;
-            }
-        }
-
-        {
-            ret := os.WriteSingleByteSimple(hb.ivLength);
-            match ret {
-                case Success(len) => totalWritten := totalWritten + len;
-                case Failure(e)  => return ret;
-            }
-        }
-
-        {
-            var bytes := UInt32ToArray(hb.frameLength);
-            ret := os.WriteSimple(bytes);
-            match ret {
-                case Success(len) => totalWritten := totalWritten + len;
-                case Failure(e)  => return ret;
-            }
-        }
-        Assume(false);
-        //reveal ReprEncryptedDataKeys();
-        assert ValidHeaderBody(hb);
-        reveal serialize();
-        ghost var serHb := serialize(hb);
-        assert totalWritten == |serHb|;
-        assert initLen+totalWritten == |os.data|;
-
-        // Turned this assertion into an assume. This assertion worked before removing the length/count from AAD/EDK datatypes
-        Assume(serHb[..totalWritten] == os.data[initLen..initLen+totalWritten]);
-
-        return Success(totalWritten);
+      ret := os.WriteSingleByteSimple(hb.typ as uint8);
+      match ret {
+        case Success(len) => totalWritten := totalWritten + len;
+        case Failure(e)  =>
+          return ret;
+      }
     }
+
+    {
+      var bytes := UInt16ToArray(hb.algorithmSuiteID as uint16);
+      ret := os.WriteSimple(bytes);
+      match ret {
+        case Success(len) => totalWritten := totalWritten + len;
+        case Failure(e)  =>
+          return ret;
+      }
+    }
+
+    {
+      ret := os.WriteSimpleSeq(hb.messageID);
+      match ret {
+        case Success(len) => totalWritten := totalWritten + len;
+        case Failure(e)  =>
+          return ret;
+      }
+    }
+
+    {
+      ret := SerializeAAD.SerializeAADImpl(os, hb.aad);
+      match ret {
+        case Success(len) => totalWritten := totalWritten + len;
+        case Failure(e)  =>
+          return ret;
+      }
+    }
+
+    {
+      ret := SerializeEDK.SerializeEDKImpl(os, hb.encryptedDataKeys);
+      match ret {
+        case Success(len) => totalWritten := totalWritten + len;
+        case Failure(e)  => return ret;
+      }
+    }
+
+    {
+      var contentType: uint8;
+      match hb.contentType {
+        case NonFramed => contentType := 0x01;
+        case Framed    => contentType := 0x02;
+      }
+      ret := os.WriteSingleByteSimple(contentType);
+      match ret {
+        case Success(len) =>
+          totalWritten := totalWritten + len;
+        case Failure(e)  =>
+          return ret;
+      }
+    }
+
+    {
+      ret := os.WriteSimpleSeq(hb.reserved);
+      match ret {
+        case Success(len) => totalWritten := totalWritten + len;
+        case Failure(e)  => return ret;
+      }
+    }
+
+    {
+      ret := os.WriteSingleByteSimple(hb.ivLength);
+      match ret {
+        case Success(len) => totalWritten := totalWritten + len;
+        case Failure(e)  => return ret;
+      }
+    }
+
+    {
+      var bytes := UInt32ToArray(hb.frameLength);
+      ret := os.WriteSimple(bytes);
+      match ret {
+        case Success(len) => totalWritten := totalWritten + len;
+        case Failure(e)  => return ret;
+      }
+    }
+    Assume(false);
+    //reveal ReprEncryptedDataKeys();
+    assert ValidHeaderBody(hb);
+    reveal Serialize();
+    ghost var serHb := Serialize(hb);
+    assert totalWritten == |serHb|;
+    assert initLen+totalWritten == |os.data|;
+
+    // Turned this assertion into an assume. This assertion worked before removing the length/count from AAD/EDK datatypes
+    Assume(serHb[..totalWritten] == os.data[initLen..initLen+totalWritten]);
+
+    return Success(totalWritten);
+  }
 }
