src/SDK/MessageHeader/SerializeAAD.dfy
@@ -5,202 +5,198 @@ include "../../Util/Streams.dfy"
 include "../../StandardLibrary/StandardLibrary.dfy"
 
 module MessageHeader.SerializeAAD {
-    import opened Definitions
-    import opened Validity
+  import opened Definitions
+  import opened Validity
 
-    import opened Streams
-    import opened StandardLibrary
-    import opened UInt = StandardLibrary.UInt
+  import Streams
+  import opened StandardLibrary
+  import opened UInt = StandardLibrary.UInt
 
-    lemma {:axiom} Assume(b : bool)
-        ensures b
+  lemma {:axiom} Assume(b: bool)
+    ensures b
 
-    function encCtxToSeqRec(kvPairs: EncCtx, i: nat): seq<uint8>
-        requires forall i :: 0 <= i < |kvPairs| ==> |kvPairs[i].0| < UINT16_LIMIT && |kvPairs[i].1| < UINT16_LIMIT
-        decreases |kvPairs| - i
-    {
-        if i < |kvPairs|
-        then
-            UInt16ToSeq(|kvPairs[i].0| as uint16) + kvPairs[i].0[..] +
-            UInt16ToSeq(|kvPairs[i].1| as uint16) + kvPairs[i].1[..] +
-            encCtxToSeqRec(kvPairs, i + 1)
-        else []
+  function EncCtxToSeqRec(kvPairs: EncCtx, i: nat): seq<uint8>
+    requires forall i :: 0 <= i < |kvPairs| ==> |kvPairs[i].0| < UINT16_LIMIT && |kvPairs[i].1| < UINT16_LIMIT
+    decreases |kvPairs| - i
+  {
+    if i < |kvPairs| then
+      UInt16ToSeq(|kvPairs[i].0| as uint16) + kvPairs[i].0[..] +
+      UInt16ToSeq(|kvPairs[i].1| as uint16) + kvPairs[i].1[..] +
+      EncCtxToSeqRec(kvPairs, i + 1)
+    else
+      []
+  }
+
+  function EncCtxToSeq(kvPairs: EncCtx): (ret: seq<uint8>)
+    requires forall i :: 0 <= i < |kvPairs| ==> |kvPairs[i].0| < UINT16_LIMIT && |kvPairs[i].1| < UINT16_LIMIT
+    ensures |ret| < UINT16_LIMIT // TODO: we need to establish that this length fits into two bytes
+  {
+    Assume(|EncCtxToSeqRec(kvPairs, 0)| < UINT16_LIMIT);  // TODO
+    EncCtxToSeqRec(kvPairs, 0)
+  }
+
+  function SerializeAAD(aad: T_AAD): seq<uint8>
+    requires ValidAAD(aad)
+  {
+    match aad {
+      case AAD(kvPairs) =>
+        Assume(forall i :: 0 <= i < |kvPairs| ==> |kvPairs[i].0| < UINT16_LIMIT && |kvPairs[i].1| < UINT16_LIMIT);
+        var encCtxSeq := EncCtxToSeq(kvPairs);
+        UInt16ToSeq(|encCtxSeq| as uint16) +
+        // It would be nicer if this could be a flatten + map as for AAD
+        UInt16ToSeq(Assume(|kvPairs| < UINT16_LIMIT); |kvPairs| as uint16) + encCtxSeq
+      case EmptyAAD() =>
+        UInt16ToSeq(0)
     }
+  }
 
-    function encCtxToSeq(kvPairs: EncCtx): (ret: seq<uint8>)
-        requires forall i :: 0 <= i < |kvPairs| ==> |kvPairs[i].0| < UINT16_LIMIT && |kvPairs[i].1| < UINT16_LIMIT
-        ensures |ret| < UINT16_LIMIT // TODO: we need to establish that this length fits into two bytes
-    {
-        Assume(|encCtxToSeqRec(kvPairs, 0)| < UINT16_LIMIT);  // TODO
-        encCtxToSeqRec(kvPairs, 0)
-    }
+  method SerializeAADImpl(os: Streams.StringWriter, aad: T_AAD) returns (ret: Result<nat>)
+    requires os.Valid() && ValidAAD(aad)
+    modifies os`data // do we need to establish non-aliasing with encryptedDataKeys here?
+    ensures os.Valid() && ValidAAD(aad)
+    //ensures old(|os.data|) <= |os.data|
+    ensures match ret
+      case Success(totalWritten) =>
+        var serAAD := SerializeAAD(aad);
+        var initLen := old(|os.data|);
+        && totalWritten == |serAAD|
+        && initLen + totalWritten == |os.data|
+        && os.data == old(os.data) + serAAD
+      case Failure(e) => true
+  {
+    var totalWritten := 0;
+    ghost var initLen := |os.data|;
+    ghost var written: seq<nat> := [initLen];
+    ghost var i := 0;
 
-    function serializeAAD(aad: T_AAD): seq<uint8>
-        requires ValidAAD(aad)
-    {
-        match aad {
-            case AAD(kvPairs) =>
-                Assume(forall i :: 0 <= i < |kvPairs| ==> |kvPairs[i].0| < UINT16_LIMIT && |kvPairs[i].1| < UINT16_LIMIT);
-                var encCtxSeq := encCtxToSeq(kvPairs);
-                UInt16ToSeq(|encCtxSeq| as uint16) +
-                // It would be nicer if this could be a flatten + map as for AAD
-                UInt16ToSeq(Assume(|kvPairs| < UINT16_LIMIT); |kvPairs| as uint16) + encCtxSeq
-            case EmptyAAD() =>
-                UInt16ToSeq(0)
+    match aad {
+      case AAD(kvPairs) =>
+        {
+          // Key Value Pairs Length (number of bytes of total AAD)
+          var length: uint16;
+          assert InBoundsKVPairs(kvPairs) ==> |kvPairs| < UINT16_LIMIT;
+          // TODO: We need to compute length here after removing length field from AAD datatype
+          Assume(forall i :: 0 <= i < |kvPairs| ==> |kvPairs[i].0| < UINT16_LIMIT && |kvPairs[i].1| < UINT16_LIMIT);
+          Assume(length == |EncCtxToSeq(kvPairs)| as uint16);
+          var bytes := UInt16ToArray(length);
+          ret := os.WriteSimple(bytes);
+          match ret {
+            case Success(len) => totalWritten := totalWritten + len;
+            case Failure(e)  => Assume(ValidAAD(aad));
+                               return ret;
+          }
+          i := i + 1;
+          written := written + [initLen + totalWritten];
+          assert written[i] - written[i-1] == bytes.Length;
+          assert written[i-1] <= written[i] <= |os.data| ==> os.data[written[i-1]..written[i]] == bytes[..];
+          Assume(ValidAAD(aad));  // TODO
+          assert totalWritten <= |SerializeAAD(aad)|;
         }
-    }
 
-    method serializeAADImpl(os: StringWriter, aad: T_AAD) returns (ret: Result<nat>)
-        requires os.Valid()
-        modifies os`data // do we need to establish non-aliasing with encryptedDataKeys here?
-        ensures os.Valid()
-        requires ValidAAD(aad)
-        ensures ValidAAD(aad)
-        ensures unchanged(os`Repr)
-        //ensures old(|os.data|) <= |os.data|
-        ensures
-            match ret
-                case Success(totalWritten) =>
-                    var serAAD := serializeAAD(aad);
-                    var initLen := old(|os.data|);
-                    && totalWritten == |serAAD|
-                    && initLen+totalWritten == |os.data|
-                    && os.data == old(os.data + serAAD)
-                case Failure(e) => true
-    {
-        var totalWritten := 0;
-        ghost var initLen := |os.data|;
-        ghost var written: seq<nat> := [initLen];
-        ghost var i := 0;
-
-        match aad {
-            case AAD(kvPairs) => {
-                {
-                    // Key Value Pairs Length (number of bytes of total AAD)
-                    var length: uint16;
-                    assert InBoundsKVPairs(kvPairs) ==> |kvPairs| < UINT16_LIMIT;
-                    // TODO: We need to compute length here after removing length field from AAD datatype
-                    Assume(forall i :: 0 <= i < |kvPairs| ==> |kvPairs[i].0| < UINT16_LIMIT && |kvPairs[i].1| < UINT16_LIMIT);
-                    Assume(length == |encCtxToSeq(kvPairs)| as uint16);
-                    var bytes := UInt16ToArray(length);
-                    ret := os.WriteSimple(bytes);
-                    match ret {
-                        case Success(len) => totalWritten := totalWritten + len;
-                        case Failure(e)  => Assume(ValidAAD(aad));
-                                          return ret;
-                    }
-                    i := i + 1;
-                    written := written + [initLen + totalWritten];
-                    assert written[i] - written[i-1] == bytes.Length;
-                    assert written[i-1] <= written[i] <= |os.data| ==> os.data[written[i-1]..written[i]] == bytes[..];
-                    Assume(ValidAAD(aad));  // TODO
-                    assert totalWritten <= |serializeAAD(aad)|;
-                }
-
-                Assume(0 < |kvPairs|);
-                assert 0 < |kvPairs|;
-                {
-                    assert InBoundsKVPairs(kvPairs) ==> |kvPairs| < UINT16_LIMIT;
-                    // Key Value Pair Count (number of key value pairs)
-                    Assume(|kvPairs| < UINT16_LIMIT);
-                    var bytes := UInt16ToArray(|kvPairs| as uint16);
-                    ret := os.WriteSimple(bytes);
-                    match ret {
-                        case Success(len) => totalWritten := totalWritten + len;
-                        case Failure(e)  => Assume(ValidAAD(aad));
-                                          return ret;
-                    }
-                    i := i + 1;
-                    written := written + [initLen + totalWritten];
-                    assert written[i] - written[i-1] == bytes.Length;
-                    assert written[i-1] <= written[i] <= |os.data| ==> os.data[written[i-1]..written[i]] == bytes[..];
-                    Assume(ValidAAD(aad));  // TODO
-                    assert totalWritten <= |serializeAAD(aad)|;
-                }
-
-                Assume(false); // TODO: verification times out after this point. I believe that we just do too many heap updates.
-
-                var j := 0;
-                while j < |kvPairs|
-                    invariant j <= |kvPairs|
-                    invariant unchanged(os`Repr)
-                    invariant InBoundsKVPairsUpTo(kvPairs, j)
-                    invariant ValidAAD(aad)
-                    invariant totalWritten <= |serializeAAD(aad)|
-                    invariant initLen+totalWritten <= |os.data|
-                    invariant serializeAAD(aad)[written[i-1]-initLen..written[i]-initLen] == os.data[written[i-1]..written[i]];
-                    //invariant serializeAAD(aad)[..totalWritten] == os.data[initLen..written[i]];
-                {
-                    {
-                        assert InBoundsKVPairsUpTo(kvPairs, j) ==> |kvPairs[j].0| < UINT16_LIMIT;
-                        var bytes := UInt16ToArray(|kvPairs[j].0| as uint16);
-                        ret := os.WriteSimple(bytes);
-                        match ret {
-                            case Success(len) => totalWritten := totalWritten + len;
-                            case Failure(e)  => return ret;
-                        }
-                        i := i + 1;
-                        written := written + [initLen + totalWritten];
-                        assert written[i] - written[i-1] == bytes.Length;
-                        assert written[i-1] <= written[i] <= |os.data| ==> os.data[written[i-1]..written[i]] == bytes[..];
-                    }
-
-                    {
-                        var bytes := kvPairs[j].0;
-                        ret := os.WriteSimpleSeq(bytes);
-                        match ret {
-                            case Success(len) => totalWritten := totalWritten + len;
-                            case Failure(e)  => return ret;
-                        }
-                        i := i + 1;
-                        written := written + [initLen + totalWritten];
-                        assert written[i] - written[i-1] == |bytes|;
-                        assert written[i-1] <= written[i] <= |os.data| ==> os.data[written[i-1]..written[i]] == bytes[..];
-                    }
-
-                    {
-                        assert InBoundsKVPairsUpTo(kvPairs, j) ==> |kvPairs[j].1| < UINT16_LIMIT;
-                        var bytes := UInt16ToSeq(|kvPairs[j].1| as uint16);
-                        ret := os.WriteSimpleSeq(bytes);
-                        match ret {
-                            case Success(len) => totalWritten := totalWritten + len;
-                            case Failure(e)  => return ret;
-                        }
-                        i := i + 1;
-                        written := written + [initLen + totalWritten];
-                        assert written[i] - written[i-1] == |bytes|;
-                        assert written[i-1] <= written[i] <= |os.data| ==> os.data[written[i-1]..written[i]] == bytes[..];
-                    }
-
-                    {
-                        var bytes := kvPairs[j].1;
-                        ret := os.WriteSimpleSeq(bytes);
-                        match ret {
-                            case Success(len) => totalWritten := totalWritten + len;
-                            case Failure(e)  => return ret;
-                        }
-                        i := i + 1;
-                        written := written + [initLen + totalWritten];
-                        assert written[i] - written[i-1] == |bytes|;
-                        assert written[i-1] <= written[i] <= |os.data| ==> os.data[written[i-1]..written[i]] == bytes[..];
-                    }
-                    j := j + 1;
-                }
-            }
-            case EmptyAAD() => {
-                var bytes := UInt16ToArray(0);
-                ret := os.WriteSimple(bytes);
-                match ret {
-                    case Success(len) => totalWritten := totalWritten + len;
-                    case Failure(e)  => Assume(ValidAAD(aad));
-                                      return ret;
-                }
-                i := i + 1;
-                written := written + [initLen + totalWritten];
-                assert written[i] - written[i-1] == 2;
-                assert written[i-1] <= written[i] <= |os.data| ==> os.data[written[i-1]..written[i]] == bytes[..];
-                Assume(ValidAAD(aad));
-            }
+        Assume(0 < |kvPairs|);
+        assert 0 < |kvPairs|;
+        {
+          assert InBoundsKVPairs(kvPairs) ==> |kvPairs| < UINT16_LIMIT;
+          // Key Value Pair Count (number of key value pairs)
+          Assume(|kvPairs| < UINT16_LIMIT);
+          var bytes := UInt16ToArray(|kvPairs| as uint16);
+          ret := os.WriteSimple(bytes);
+          match ret {
+            case Success(len) => totalWritten := totalWritten + len;
+            case Failure(e)  => Assume(ValidAAD(aad));
+                               return ret;
+          }
+          i := i + 1;
+          written := written + [initLen + totalWritten];
+          assert written[i] - written[i-1] == bytes.Length;
+          assert written[i-1] <= written[i] <= |os.data| ==> os.data[written[i-1]..written[i]] == bytes[..];
+          Assume(ValidAAD(aad));  // TODO
+          assert totalWritten <= |SerializeAAD(aad)|;
         }
+
+        Assume(false); // TODO: verification times out after this point. I believe that we just do too many heap updates.
+
+        var j := 0;
+        while j < |kvPairs|
+          invariant j <= |kvPairs|
+          invariant unchanged(os`Repr)
+          invariant InBoundsKVPairsUpTo(kvPairs, j)
+          invariant ValidAAD(aad)
+          invariant totalWritten <= |SerializeAAD(aad)|
+          invariant initLen+totalWritten <= |os.data|
+          invariant SerializeAAD(aad)[written[i-1]-initLen..written[i]-initLen] == os.data[written[i-1]..written[i]];
+          //invariant SerializeAAD(aad)[..totalWritten] == os.data[initLen..written[i]];
+        {
+          {
+            assert InBoundsKVPairsUpTo(kvPairs, j) ==> |kvPairs[j].0| < UINT16_LIMIT;
+            var bytes := UInt16ToArray(|kvPairs[j].0| as uint16);
+            ret := os.WriteSimple(bytes);
+            match ret {
+              case Success(len) => totalWritten := totalWritten + len;
+              case Failure(e)  => return ret;
+            }
+            i := i + 1;
+            written := written + [initLen + totalWritten];
+            assert written[i] - written[i-1] == bytes.Length;
+            assert written[i-1] <= written[i] <= |os.data| ==> os.data[written[i-1]..written[i]] == bytes[..];
+          }
+
+          {
+            var bytes := kvPairs[j].0;
+            ret := os.WriteSimpleSeq(bytes);
+            match ret {
+              case Success(len) => totalWritten := totalWritten + len;
+              case Failure(e)  => return ret;
+            }
+            i := i + 1;
+            written := written + [initLen + totalWritten];
+            assert written[i] - written[i-1] == |bytes|;
+            assert written[i-1] <= written[i] <= |os.data| ==> os.data[written[i-1]..written[i]] == bytes[..];
+          }
+
+          {
+            assert InBoundsKVPairsUpTo(kvPairs, j) ==> |kvPairs[j].1| < UINT16_LIMIT;
+            var bytes := UInt16ToSeq(|kvPairs[j].1| as uint16);
+            ret := os.WriteSimpleSeq(bytes);
+            match ret {
+              case Success(len) => totalWritten := totalWritten + len;
+              case Failure(e)  => return ret;
+            }
+            i := i + 1;
+            written := written + [initLen + totalWritten];
+            assert written[i] - written[i-1] == |bytes|;
+            assert written[i-1] <= written[i] <= |os.data| ==> os.data[written[i-1]..written[i]] == bytes[..];
+          }
+
+          {
+            var bytes := kvPairs[j].1;
+            ret := os.WriteSimpleSeq(bytes);
+            match ret {
+              case Success(len) => totalWritten := totalWritten + len;
+              case Failure(e)  => return ret;
+            }
+            i := i + 1;
+            written := written + [initLen + totalWritten];
+            assert written[i] - written[i-1] == |bytes|;
+            assert written[i-1] <= written[i] <= |os.data| ==> os.data[written[i-1]..written[i]] == bytes[..];
+          }
+
+          j := j + 1;
+        }
+
+      case EmptyAAD() =>
+        var bytes := UInt16ToArray(0);
+        ret := os.WriteSimple(bytes);
+        match ret {
+          case Success(len) => totalWritten := totalWritten + len;
+          case Failure(e)  => Assume(ValidAAD(aad));
+                             return ret;
+        }
+        i := i + 1;
+        written := written + [initLen + totalWritten];
+        assert written[i] - written[i-1] == 2;
+        assert written[i-1] <= written[i] <= |os.data| ==> os.data[written[i-1]..written[i]] == bytes[..];
+        Assume(ValidAAD(aad));
     }
+  }
 }
