src/SDK/MessageHeader/SerializeEDK.dfy
@@ -5,187 +5,184 @@ include "../../Util/Streams.dfy"
 include "../../StandardLibrary/StandardLibrary.dfy"
 
 module MessageHeader.SerializeEDK {
-    import opened Definitions
-    import opened Validity
+  import opened Definitions
+  import opened Validity
 
-    import opened Streams
-    import opened StandardLibrary
-    import opened UInt = StandardLibrary.UInt
+  import Streams
+  import opened StandardLibrary
+  import opened UInt = StandardLibrary.UInt
 
-    lemma {:axiom} Assume(b: bool) ensures b
+  lemma {:axiom} Assume(b: bool)
+    ensures b
 
-    // Alternative w/o flatten/map
-    function serializeEDKEntries(entries: seq<EDKEntry>): seq<uint8>
-        requires forall i :: 0 <= i < |entries| ==> entries[i].Valid()
+  // Alternative w/o flatten/map
+  function SerializeEDKEntries(entries: seq<EDKEntry>): seq<uint8>
+    requires forall i :: 0 <= i < |entries| ==> entries[i].Valid()
+  {
+    if entries == [] then
+      []
+    else
+      var entry := entries[0];
+      UInt16ToSeq(|entry.providerID| as uint16)   + StringToByteSeq(entry.providerID) +
+      UInt16ToSeq(|entry.providerInfo| as uint16) + entry.providerInfo +
+      UInt16ToSeq(|entry.ciphertext| as uint16)   + entry.ciphertext +
+      SerializeEDKEntries(entries[1..])
+  }
+
+  function SerializeEDK(encryptedDataKeys: T_EncryptedDataKeys): seq<uint8>
+    requires ValidEncryptedDataKeys(encryptedDataKeys)
+  {
+    Assume(|encryptedDataKeys.entries| < UINT16_LIMIT);
+    Assume(forall i :: 0 <= i < |encryptedDataKeys.entries| ==> encryptedDataKeys.entries[i].Valid());
+    UInt16ToSeq(|encryptedDataKeys.entries| as uint16) +
+    SerializeEDKEntries(encryptedDataKeys.entries)
+  }
+
+  method SerializeEDKImpl(os: Streams.StringWriter, encryptedDataKeys: T_EncryptedDataKeys) returns (ret: Result<nat>)
+    requires os.Valid() && ValidEncryptedDataKeys(encryptedDataKeys)
+    modifies os`data
+    ensures os.Valid() && ValidEncryptedDataKeys(encryptedDataKeys)
+    //ensures old(|os.data|) <= |os.data|
+    ensures match ret
+      case Success(totalWritten) =>
+        var serEDK := SerializeEDK(encryptedDataKeys);
+        var initLen := old(|os.data|);
+        && totalWritten == |serEDK|
+        && initLen + totalWritten == |os.data|
+        && os.data == old(os.data) + serEDK
+      case Failure(e) => true
+  {
+    Assume(false);  // TODO: turned off verification for now
+    var totalWritten: nat := 0;
+    ghost var initLen := |os.data|;
+    ghost var prevPos: nat := initLen;
+    ghost var currPos: nat := initLen;
+
     {
-        if entries == []
-        then []
-        else
-            var entry := entries[0];
-            UInt16ToSeq(|entry.providerID| as uint16)   + StringToByteSeq(entry.providerID) +
-            UInt16ToSeq(|entry.providerInfo| as uint16) + entry.providerInfo +
-            UInt16ToSeq(|entry.ciphertext| as uint16)   + entry.ciphertext +
-            serializeEDKEntries(entries[1..])
+      Assume(|encryptedDataKeys.entries| < UINT16_LIMIT);
+      var bytes := UInt16ToArray(|encryptedDataKeys.entries| as uint16);
+      ret := os.WriteSimple(bytes);
+      match ret {
+        case Success(len) => totalWritten := totalWritten + len;
+        case Failure(e)  => return ret;
+      }
+      prevPos := currPos;
+      currPos := initLen + totalWritten;
+      assert currPos - prevPos == bytes.Length;
+      assert prevPos <= currPos <= |os.data| ==> os.data[prevPos..currPos] == bytes[..];
+      assert totalWritten <= |SerializeEDK(encryptedDataKeys)|;
     }
 
-    function serializeEDK(encryptedDataKeys: T_EncryptedDataKeys): seq<uint8>
-        requires ValidEncryptedDataKeys(encryptedDataKeys)
+    var j := 0;
+    ghost var written: seq<nat> := [currPos, currPos];
+    while j < |encryptedDataKeys.entries|
+      invariant j <= |encryptedDataKeys.entries|
+      invariant j < |written|
+      invariant unchanged(os`Repr)
+      invariant InBoundsEncryptedDataKeysUpTo(encryptedDataKeys.entries, j)
+      invariant ValidEncryptedDataKeys(encryptedDataKeys)
+      invariant initLen + totalWritten == currPos
+      invariant 0 <= initLen <= prevPos <= currPos <= |os.data|
+      invariant forall k :: 0 <= k < |written| ==> initLen <= written[k] <= |os.data|
+      invariant currPos-initLen <= |SerializeEDK(encryptedDataKeys)|
+      invariant SerializeEDK(encryptedDataKeys)[..currPos-initLen] == os.data[initLen..currPos]
+      invariant SerializeEDK(encryptedDataKeys)[prevPos-initLen..currPos-initLen] == os.data[prevPos..currPos];
+      invariant 1 <= j ==> os.data[initLen..written[j]] == os.data[initLen..written[j-1]] + SerializeEDKEntries(encryptedDataKeys.entries[..j])
     {
-        Assume(|encryptedDataKeys.entries| < UINT16_LIMIT);
-        Assume(forall i :: 0 <= i < |encryptedDataKeys.entries| ==> encryptedDataKeys.entries[i].Valid());
-        UInt16ToSeq(|encryptedDataKeys.entries| as uint16) +
-        serializeEDKEntries(encryptedDataKeys.entries)
-    }
-
-    method serializeEDKImpl(os: StringWriter, encryptedDataKeys: T_EncryptedDataKeys) returns (ret: Result<nat>)
-        requires os.Valid()
-        modifies os`data
-        ensures os.Valid()
-        requires ValidEncryptedDataKeys(encryptedDataKeys)
-        ensures ValidEncryptedDataKeys(encryptedDataKeys)
-        ensures unchanged(os`Repr)
-        //ensures old(|os.data|) <= |os.data|
-        ensures
-            match ret
-                case Success(totalWritten) =>
-                    var serEDK := serializeEDK(encryptedDataKeys);
-                    var initLen := old(|os.data|);
-                    && totalWritten == |serEDK|
-                    && initLen+totalWritten == |os.data|
-                    && os.data == old(os.data + serEDK)
-                case Failure(e) => true
-    {
-        Assume(false);  // TODO: turned off verification for now
-        var totalWritten: nat := 0;
-        ghost var initLen := |os.data|;
-        ghost var prevPos: nat := initLen;
-        ghost var currPos: nat := initLen;
-
-        {
-            Assume(|encryptedDataKeys.entries| < UINT16_LIMIT);
-            var bytes := UInt16ToArray(|encryptedDataKeys.entries| as uint16);
-            ret := os.WriteSimple(bytes);
-            match ret {
-                case Success(len) => totalWritten := totalWritten + len;
-                case Failure(e)  => return ret;
-            }
-            prevPos := currPos;
-            currPos := initLen + totalWritten;
-            assert currPos - prevPos == bytes.Length;
-            assert prevPos <= currPos <= |os.data| ==> os.data[prevPos..currPos] == bytes[..];
-            assert totalWritten <= |serializeEDK(encryptedDataKeys)|;
+      var entry := encryptedDataKeys.entries[j];
+      {
+        Assume(|entry.providerID| < UINT16_LIMIT);
+        var bytes := UInt16ToArray(|entry.providerID| as uint16);
+        ret := os.WriteSimple(bytes);
+        match ret {
+          case Success(len) => totalWritten := totalWritten + len;
+          case Failure(e)  => return ret;
         }
+        prevPos := currPos;
+        currPos := initLen + totalWritten;
+        Assume(prevPos <= currPos <= |os.data| ==> os.data[prevPos..currPos] == bytes[..]);
+        assert prevPos <= currPos <= |os.data| ==> os.data[prevPos..currPos] == bytes[..];
+      }
 
-        var j := 0;
-        ghost var written: seq<nat> := [currPos, currPos];
-        while j < |encryptedDataKeys.entries|
-            invariant j <= |encryptedDataKeys.entries|
-            invariant j < |written|
-            invariant unchanged(os`Repr)
-            invariant InBoundsEncryptedDataKeysUpTo(encryptedDataKeys.entries, j)
-            invariant ValidEncryptedDataKeys(encryptedDataKeys)
-            invariant initLen + totalWritten == currPos
-            invariant 0 <= initLen <= prevPos <= currPos <= |os.data|
-            invariant forall k :: 0 <= k < |written| ==> initLen <= written[k] <= |os.data|
-            invariant currPos-initLen <= |serializeEDK(encryptedDataKeys)|
-            invariant serializeEDK(encryptedDataKeys)[..currPos-initLen] == os.data[initLen..currPos]
-            invariant serializeEDK(encryptedDataKeys)[prevPos-initLen..currPos-initLen] == os.data[prevPos..currPos];
-            invariant 1 <= j ==> os.data[initLen..written[j]] == os.data[initLen..written[j-1]] + serializeEDKEntries(encryptedDataKeys.entries[..j])
-        {
-            var entry := encryptedDataKeys.entries[j];
-            {
-                Assume(|entry.providerID| < UINT16_LIMIT);
-                var bytes := UInt16ToArray(|entry.providerID| as uint16);
-                ret := os.WriteSimple(bytes);
-                match ret {
-                    case Success(len) => totalWritten := totalWritten + len;
-                    case Failure(e)  => return ret;
-                }
-                prevPos := currPos;
-                currPos := initLen + totalWritten;
-                Assume(prevPos <= currPos <= |os.data| ==> os.data[prevPos..currPos] == bytes[..]);
-                assert prevPos <= currPos <= |os.data| ==> os.data[prevPos..currPos] == bytes[..];
-            }
-
-            {
-                var bytes := StringToByteSeq(entry.providerID);
-                ret := os.WriteSimpleSeq(bytes);
-                match ret {
-                    case Success(len) => totalWritten := totalWritten + len;
-                    case Failure(e)  => return ret;
-                }
-                prevPos := currPos;
-                currPos := initLen + totalWritten;
-                assert currPos - prevPos == |bytes|;
-                Assume(prevPos <= currPos <= |os.data| ==> os.data[prevPos..currPos] == bytes[..]);
-                assert prevPos <= currPos <= |os.data| ==> os.data[prevPos..currPos] == bytes[..];
-            }
-
-            {
-                Assume(|entry.providerInfo| < UINT16_LIMIT);
-                var bytes := UInt16ToArray(|entry.providerInfo| as uint16);
-                ret := os.WriteSimple(bytes);
-                match ret {
-                    case Success(len) => totalWritten := totalWritten + len;
-                    case Failure(e)  => return ret;
-                }
-                prevPos := currPos;
-                currPos := initLen + totalWritten;
-                assert currPos - prevPos == bytes.Length;
-                Assume(prevPos <= currPos <= |os.data| ==> os.data[prevPos..currPos] == bytes[..]);
-                assert prevPos <= currPos <= |os.data| ==> os.data[prevPos..currPos] == bytes[..];
-            }
-
-            {
-                var bytes := entry.providerInfo;
-                ret := os.WriteSimpleSeq(bytes);
-                match ret {
-                    case Success(len) => totalWritten := totalWritten + len;
-                    case Failure(e)  => return ret;
-                }
-                prevPos := currPos;
-                currPos := initLen + totalWritten;
-                assert currPos - prevPos == |bytes|;
-                Assume(prevPos <= currPos <= |os.data| ==> os.data[prevPos..currPos] == bytes[..]);
-                assert prevPos <= currPos <= |os.data| ==> os.data[prevPos..currPos] == bytes[..];
-            }
-
-            {
-                Assume(|entry.ciphertext| < UINT16_LIMIT);
-                var bytes := UInt16ToArray(|entry.ciphertext| as uint16);
-                ret := os.WriteSimple(bytes);
-                match ret {
-                    case Success(len) => totalWritten := totalWritten + len;
-                    case Failure(e)  => return ret;
-                }
-                prevPos := currPos;
-                currPos := initLen + totalWritten;
-                assert currPos - prevPos == bytes.Length;
-                Assume(prevPos <= currPos <= |os.data| ==> os.data[prevPos..currPos] == bytes[..]);
-                assert prevPos <= currPos <= |os.data| ==> os.data[prevPos..currPos] == bytes[..];
-            }
-
-            {
-                var bytes := entry.ciphertext;
-                ret := os.WriteSimpleSeq(bytes);
-                match ret {
-                    case Success(len) => totalWritten := totalWritten + len;
-                    case Failure(e)  => return ret;
-                }
-                prevPos := currPos;
-                currPos := initLen + totalWritten;
-                assert currPos - prevPos == |bytes|;
-                Assume(prevPos <= currPos <= |os.data| ==> os.data[prevPos..currPos] == bytes[..]);
-                assert prevPos <= currPos <= |os.data| ==> os.data[prevPos..currPos] == bytes[..];
-            }
-            written := written + [currPos];
-            j := j + 1;
-            Assume(ValidEncryptedDataKeys(encryptedDataKeys));
+      {
+        var bytes := StringToByteSeq(entry.providerID);
+        ret := os.WriteSimpleSeq(bytes);
+        match ret {
+          case Success(len) => totalWritten := totalWritten + len;
+          case Failure(e)  => return ret;
         }
+        prevPos := currPos;
+        currPos := initLen + totalWritten;
+        assert currPos - prevPos == |bytes|;
+        Assume(prevPos <= currPos <= |os.data| ==> os.data[prevPos..currPos] == bytes[..]);
+        assert prevPos <= currPos <= |os.data| ==> os.data[prevPos..currPos] == bytes[..];
+      }
 
-        Assume(totalWritten == |serializeEDK(encryptedDataKeys)|);
-        Assume(initLen+totalWritten == |os.data|);
-        Assume(os.data == old(os.data) + serializeEDK(encryptedDataKeys));
-        return Success(totalWritten);
+      {
+        Assume(|entry.providerInfo| < UINT16_LIMIT);
+        var bytes := UInt16ToArray(|entry.providerInfo| as uint16);
+        ret := os.WriteSimple(bytes);
+        match ret {
+          case Success(len) => totalWritten := totalWritten + len;
+          case Failure(e)  => return ret;
+        }
+        prevPos := currPos;
+        currPos := initLen + totalWritten;
+        assert currPos - prevPos == bytes.Length;
+        Assume(prevPos <= currPos <= |os.data| ==> os.data[prevPos..currPos] == bytes[..]);
+        assert prevPos <= currPos <= |os.data| ==> os.data[prevPos..currPos] == bytes[..];
+      }
+
+      {
+        var bytes := entry.providerInfo;
+        ret := os.WriteSimpleSeq(bytes);
+        match ret {
+          case Success(len) => totalWritten := totalWritten + len;
+          case Failure(e)  => return ret;
+        }
+        prevPos := currPos;
+        currPos := initLen + totalWritten;
+        assert currPos - prevPos == |bytes|;
+        Assume(prevPos <= currPos <= |os.data| ==> os.data[prevPos..currPos] == bytes[..]);
+        assert prevPos <= currPos <= |os.data| ==> os.data[prevPos..currPos] == bytes[..];
+      }
+
+      {
+        Assume(|entry.ciphertext| < UINT16_LIMIT);
+        var bytes := UInt16ToArray(|entry.ciphertext| as uint16);
+        ret := os.WriteSimple(bytes);
+        match ret {
+          case Success(len) => totalWritten := totalWritten + len;
+          case Failure(e)  => return ret;
+        }
+        prevPos := currPos;
+        currPos := initLen + totalWritten;
+        assert currPos - prevPos == bytes.Length;
+        Assume(prevPos <= currPos <= |os.data| ==> os.data[prevPos..currPos] == bytes[..]);
+        assert prevPos <= currPos <= |os.data| ==> os.data[prevPos..currPos] == bytes[..];
+      }
+
+      {
+        var bytes := entry.ciphertext;
+        ret := os.WriteSimpleSeq(bytes);
+        match ret {
+          case Success(len) => totalWritten := totalWritten + len;
+          case Failure(e)  => return ret;
+        }
+        prevPos := currPos;
+        currPos := initLen + totalWritten;
+        assert currPos - prevPos == |bytes|;
+        Assume(prevPos <= currPos <= |os.data| ==> os.data[prevPos..currPos] == bytes[..]);
+        assert prevPos <= currPos <= |os.data| ==> os.data[prevPos..currPos] == bytes[..];
+      }
+      written := written + [currPos];
+      j := j + 1;
+      Assume(ValidEncryptedDataKeys(encryptedDataKeys));
     }
+
+    Assume(totalWritten == |SerializeEDK(encryptedDataKeys)|);
+    Assume(initLen+totalWritten == |os.data|);
+    Assume(os.data == old(os.data) + SerializeEDK(encryptedDataKeys));
+    return Success(totalWritten);
+  }
 }
