src/SDK/MessageHeader/Deserialize.dfy
@@ -7,7 +7,6 @@ include "../../Util/Streams.dfy"
 include "../../StandardLibrary/StandardLibrary.dfy"
 include "../../Util/UTF8.dfy"
 
-
 /*
  * The message header deserialization
  *
@@ -15,588 +14,580 @@ include "../../Util/UTF8.dfy"
  * When encountering an error, we stop and return it immediately, leaving the remaining inputs on the stream
  */
 module MessageHeader.Deserialize {
-    import opened Definitions
-    import opened Validity
-    import opened Utils
+  import opened Definitions
+  import opened Validity
+  import Utils
 
-    import AlgorithmSuite
-    import opened Streams
-    import opened StandardLibrary
-    import opened UInt = StandardLibrary.UInt
-    import opened UTF8
+  import AlgorithmSuite
+  import Streams
+  import opened StandardLibrary
+  import opened UInt = StandardLibrary.UInt
+  import UTF8
 
-    lemma {:axiom} Assume(b : bool) ensures b
+  lemma {:axiom} Assume(b: bool)
+    ensures b
 
-    /*
-     * Message header-specific
-     */
+  /*
+   * Message header-specific
+   */
 
-    method deserializeVersion(is: StringReader) returns (ret: Result<T_Version>)
-        requires is.Valid()
-        modifies is
-        ensures is.Valid()
+  method DeserializeVersion(is: Streams.StringReader) returns (ret: Result<T_Version>)
+    requires is.Valid()
+    modifies is
+    ensures is.Valid()
+  {
+    var res := Utils.ReadFixedLengthFromStreamOrFail(is, 1);
+    match res {
+      case Success(version) =>
+        if version[0] == 0x01 {
+          return Success(version[0] as T_Version);
+        } else {
+          return Failure("Deserialization Error: Version not supported.");
+        }
+      case Failure(e) => return Failure(e);
+    }
+  }
+
+  method DeserializeType(is: Streams.StringReader) returns (ret: Result<T_Type>)
+    requires is.Valid()
+    modifies is
+    ensures is.Valid()
+  {
+    var res := Utils.ReadFixedLengthFromStreamOrFail(is, 1);
+    match res {
+      case Success(typ) =>
+        if typ[0] == 0x80 {
+          return Success(typ[0] as T_Type);
+        } else {
+          return Failure("Deserialization Error: Type not supported.");
+        }
+      case Failure(e) => return Failure(e);
+    }
+  }
+
+  method DeserializeAlgorithmSuiteID(is: Streams.StringReader) returns (ret: Result<AlgorithmSuite.ID>)
+    requires is.Valid()
+    modifies is
+    ensures is.Valid()
+    ensures match ret
+      case Success(algorithmSuiteID) => ValidAlgorithmID(algorithmSuiteID)
+      case Failure(_) => true
+  {
+    var res := Utils.ReadFixedLengthFromStreamOrFail(is, 2);
+    match res {
+      case Success(algorithmSuiteID) =>
+        var asid := ArrayToUInt16(algorithmSuiteID);
+        if asid in AlgorithmSuite.validIDs {
+          return Success(asid as AlgorithmSuite.ID);
+        } else {
+          return Failure("Deserialization Error: Algorithm suite not supported.");
+        }
+      case Failure(e) => return Failure(e);
+    }
+  }
+
+  // TODO:
+  predicate method IsValidMsgID (candidateID: array<uint8>)
+    requires candidateID.Length == 16
+    ensures ValidMessageId(candidateID[..])
+  {
+    true
+  }
+
+  method DeserializeMsgID(is: Streams.StringReader) returns (ret: Result<T_MessageID>)
+    requires is.Valid()
+    modifies is
+    ensures is.Valid()
+    ensures match ret
+      case Success(msgId) => ValidMessageId(msgId)
+      case Failure(_) => true
+  {
+    var res := Utils.ReadFixedLengthFromStreamOrFail(is, 16);
+    match res {
+      case Success(msgId) =>
+        if IsValidMsgID(msgId) {
+          return Success(msgId[..]);
+        } else {
+          return Failure("Deserialization Error: Not a valid Message ID.");
+        }
+      case Failure(e) => return Failure(e);
+    }
+  }
+
+  method DeserializeUTF8(is: Streams.StringReader, n: nat) returns (ret: Result<array<uint8>>)
+    requires is.Valid()
+    modifies is
+    ensures is.Valid()
+    ensures match ret
+      case Success(bytes) =>
+        && bytes.Length == n
+        && UTF8.ValidUTF8(bytes)
+        && fresh(bytes)
+      case Failure(_) => true
+  {
+    ret := Utils.ReadFixedLengthFromStreamOrFail(is, n);
+    match ret {
+      case Success(bytes) =>
+        if UTF8.ValidUTF8(bytes) {
+          return ret;
+        } else {
+          return Failure("Deserialization Error: Not a valid UTF8 string.");
+        }
+      case Failure(e) => return ret;
+    }
+  }
+
+  method DeserializeUnrestricted(is: Streams.StringReader, n: nat) returns (ret: Result<array<uint8>>)
+    requires is.Valid()
+    modifies is
+    ensures is.Valid()
+    ensures match ret
+      case Success(bytes) =>
+        && bytes.Length == n
+        && fresh(bytes)
+      case Failure(_) => true
+  {
+    ret := Utils.ReadFixedLengthFromStreamOrFail(is, n);
+  }
+
+  // TODO: Probably this should be factored out into EncCtx at some point
+  method DeserializeAAD(is: Streams.StringReader) returns (ret: Result<T_AAD>)
+    requires is.Valid()
+    modifies is
+    ensures is.Valid()
+    ensures match ret
+      case Success(aad) =>
+        && ValidAAD(aad)
+      case Failure(_) => true
+  {
+    reveal ValidAAD();
+    var kvPairsLength: uint16;
     {
-        var res := readFixedLengthFromStreamOrFail(is, 1);
+      var res := DeserializeUnrestricted(is, 2);
+      match res {
+        case Success(bytes) => kvPairsLength := ArrayToUInt16(bytes);
+        case Failure(e) => return Failure(e);
+      }
+    }
+    if kvPairsLength == 0 {
+      return Success(EmptyAAD);
+    }
+    var totalBytesRead := 0;
+
+    var kvPairsCount: uint16;
+    {
+      var res := DeserializeUnrestricted(is, 2);
+      match res {
+        case Success(bytes) =>
+          kvPairsCount := ArrayToUInt16(bytes);
+          totalBytesRead := totalBytesRead + bytes.Length;
+          if kvPairsLength > 0 && kvPairsCount == 0 {
+            return Failure("Deserialization Error: Key value pairs count is 0.");
+          }
+          assert kvPairsLength > 0 ==> kvPairsCount > 0;
+        case Failure(e) => return Failure(e);
+      }
+    }
+
+    // TODO: declare this array, make kvPairs a ghost, maintain invariant that sequence is a prefix of the array:
+    // var kvPairsArray: array<(seq<uint8>, seq<uint8>)> := new [kvPairsCount];
+    var kvPairs: seq<(seq<uint8>, seq<uint8>)> := [];
+    assert kvPairsCount > 0;
+
+    var i := 0;
+    while i < kvPairsCount
+      invariant is.Valid()
+      invariant |kvPairs| == i as int
+      invariant i <= kvPairsCount
+      invariant InBoundsKVPairsUpTo(kvPairs, i as nat)
+      invariant Utils.SortedKVPairsUpTo(kvPairs, i as nat)
+      invariant forall j :: 0 <= j < i ==> UTF8.ValidUTF8Seq(kvPairs[j].0)
+      invariant forall j :: 0 <= j < i ==> UTF8.ValidUTF8Seq(kvPairs[j].1)
+    {
+      var keyLength: uint16;
+      {
+        var res := DeserializeUnrestricted(is, 2);
         match res {
-            case Success(version) =>
-                if version[0] == 0x01 {
-                    return Success(version[0] as T_Version);
-                } else {
-                    return Failure("Deserialization Error: Version not supported.");
-                }
-            case Failure(e) => return Failure(e);
+          case Success(bytes) =>
+            keyLength := ArrayToUInt16(bytes);
+            totalBytesRead := totalBytesRead + bytes.Length;
+          case Failure(e) => return Failure(e);
         }
-    }
+      }
 
-    method deserializeType(is: StringReader) returns (ret: Result<T_Type>)
-        requires is.Valid()
-        modifies is
-        ensures is.Valid()
-    {
-        var res := readFixedLengthFromStreamOrFail(is, 1);
+      var key: seq<uint8>;
+      {
+        var res := DeserializeUTF8(is, keyLength as nat);
         match res {
-            case Success(typ) =>
-                if typ[0] == 0x80 {
-                    return Success(typ[0] as T_Type);
-                } else {
-                    return Failure("Deserialization Error: Type not supported.");
-                }
-            case Failure(e) => return Failure(e);
+          case Success(bytes) =>
+            UTF8.ValidUTF8ArraySeq(bytes);
+            key := bytes[..];
+            totalBytesRead := totalBytesRead + bytes.Length;
+          case Failure(e) => return Failure(e);
         }
-    }
+      }
+      assert |key| < UINT16_LIMIT;
+      assert UTF8.ValidUTF8Seq(key);
 
-    method deserializeAlgorithmSuiteID(is: StringReader) returns (ret: Result<AlgorithmSuite.ID>)
-        requires is.Valid()
-        modifies is
-        ensures
-            match ret
-                case Success(algorithmSuiteID) => ValidAlgorithmID(algorithmSuiteID)
-                case Failure(_) => true
-        ensures is.Valid()
-    {
-        var res := readFixedLengthFromStreamOrFail(is, 2);
+      var valueLength: uint16;
+      {
+        var res := DeserializeUnrestricted(is, 2);
         match res {
-            case Success(algorithmSuiteID) =>
-                var asid := ArrayToUInt16(algorithmSuiteID);
-                if asid in AlgorithmSuite.validIDs {
-                    return Success(asid as AlgorithmSuite.ID);
-                } else {
-                    return Failure("Deserialization Error: Algorithm suite not supported.");
-                }
-            case Failure(e) => return Failure(e);
+          case Success(bytes) =>
+            valueLength := ArrayToUInt16(bytes);
+            totalBytesRead := totalBytesRead + bytes.Length;
+          case Failure(e) => return Failure(e);
         }
-    }
+      }
 
-    // TODO:
-    predicate method isValidMsgID (candidateID: array<uint8>)
-        requires candidateID.Length == 16
-        ensures ValidMessageId(candidateID[..])
-    {
-        true
-    }
-    method deserializeMsgID(is: StringReader) returns (ret: Result<T_MessageID>)
-        requires is.Valid()
-        modifies is
-        ensures
-            match ret
-                case Success(msgId) => ValidMessageId(msgId)
-                case Failure(_) => true
-        ensures is.Valid()
-    {
-        var res := readFixedLengthFromStreamOrFail(is, 16);
+      var value: seq<uint8>;
+      {
+        var res := DeserializeUTF8(is, valueLength as nat);
         match res {
-            case Success(msgId) =>
-                if isValidMsgID(msgId) {
-                    return Success(msgId[..]);
-                } else {
-                    return Failure("Deserialization Error: Not a valid Message ID.");
-                }
-            case Failure(e) => return Failure(e);
+          case Success(bytes) =>
+            UTF8.ValidUTF8ArraySeq(bytes);
+            value := bytes[..];
+            totalBytesRead := totalBytesRead + bytes.Length;
+          case Failure(e) => return Failure(e);
         }
+      }
+      assert |value| < UINT16_LIMIT;
+      assert UTF8.ValidUTF8Seq(value);
+
+      // check for sortedness by key
+      if i != 0 && !LexCmpSeqs(kvPairs[i - 1].0, key, UInt8Less) {
+        return Failure("Deserialization Error: Key-value pairs must be sorted by key.");
+      }
+      kvPairs := kvPairs + [(key, value)];
+      assert Utils.SortedKVPairsUpTo(kvPairs, (i+1) as nat);
+      i := i + 1;
+    }
+    if (kvPairsLength as nat) != totalBytesRead {
+      return Failure("Deserialization Error: Bytes actually read differs from bytes supposed to be read.");
+    }
+    return Success(AAD(kvPairs));
+  }
+
+  // TODO: Probably this should be factored out into EDK at some point
+  method DeserializeEncryptedDataKeys(is: Streams.StringReader, ghost aad: T_AAD) returns (ret: Result<T_EncryptedDataKeys>)
+    requires is.Valid()
+    modifies is
+    ensures is.Valid()
+    ensures match ret
+      case Success(edks) =>
+        && ValidEncryptedDataKeys(edks)
+      case Failure(_)   => true
+  {
+    reveal ValidEncryptedDataKeys();
+    var edkCount: uint16;
+    var res := DeserializeUnrestricted(is, 2);
+    match res {
+      case Success(bytes) => edkCount := ArrayToUInt16(bytes);
+      case Failure(e)    => return Failure(e);
     }
 
-    method deserializeUTF8(is: StringReader, n: nat) returns (ret: Result<array<uint8>>)
-        requires is.Valid()
-        modifies is
-        ensures
-            match ret
-                case Success(bytes) =>
-                    && bytes.Length == n
-                    && ValidUTF8(bytes)
-                    && fresh(bytes)
-                case Failure(_) => true
-        ensures is.Valid()
+    if edkCount == 0 {
+      return Failure("Deserialization Error: Encrypted data key count must be > 0.");
+    }
+
+    var edkEntries: seq<EDKEntry> := [];
+    var i := 0;
+    while i < edkCount
+      invariant is.Valid()
+      invariant i <= edkCount
+      invariant InBoundsEncryptedDataKeys(edkEntries)
     {
-        ret := readFixedLengthFromStreamOrFail(is, n);
-        match ret {
-            case Success(bytes) =>
-                if ValidUTF8(bytes) {
-                    return ret;
-                } else {
-                    return Failure("Deserialization Error: Not a valid UTF8 string.");
-                }
-            case Failure(e) => return ret;
-        }
+      // Key provider ID
+      var keyProviderIDLength: uint16;
+      res := DeserializeUnrestricted(is, 2);
+      match res {
+        case Success(bytes) => keyProviderIDLength := ArrayToUInt16(bytes);
+        case Failure(e)    => return Failure(e);
+      }
+
+      var keyProviderID: string;
+      res := DeserializeUTF8(is, keyProviderIDLength as nat);
+      match res {
+        case Success(bytes) => keyProviderID := ByteSeqToString(bytes[..]);
+        case Failure(e)    => return Failure(e);
+      }
+
+      // Key provider info
+      var keyProviderInfoLength: uint16;
+      res := DeserializeUnrestricted(is, 2);
+      match res {
+        case Success(bytes) => keyProviderInfoLength := ArrayToUInt16(bytes);
+        case Failure(e)    => return Failure(e);
+      }
+
+      var keyProviderInfo: seq<uint8>;
+      res := DeserializeUnrestricted(is, keyProviderInfoLength as nat);
+      match res {
+        case Success(bytes) => keyProviderInfo := bytes[..];
+        case Failure(e)    => return Failure(e);
+      }
+
+      // Encrypted data key
+      var edkLength: uint16;
+      res := DeserializeUnrestricted(is, 2);
+      match res {
+        case Success(bytes) => edkLength := ArrayToUInt16(bytes);
+        case Failure(e)    => return Failure(e);
+      }
+
+      var edk: seq<uint8>;
+      res := DeserializeUnrestricted(is, edkLength as nat);
+      match res {
+        case Success(bytes) => edk := bytes[..];
+        case Failure(e)    => return Failure(e);
+      }
+
+      edkEntries := edkEntries + [Materials.EncryptedDataKey(keyProviderID, keyProviderInfo, edk)];
+      i := i + 1;
     }
 
-    method deserializeUnrestricted(is: StringReader, n: nat) returns (ret: Result<array<uint8>>)
-        requires is.Valid()
-        modifies is
-        ensures
-            match ret
-                case Success(bytes) =>
-                    && bytes.Length == n
-                    && fresh(bytes)
-                case Failure(_) => true
-        ensures is.Valid()
+    var edks := EncryptedDataKeys(edkEntries);
+    return Success(edks);
+  }
+
+  method DeserializeContentType(is: Streams.StringReader) returns (ret: Result<T_ContentType>)
+    requires is.Valid()
+    modifies is
+    ensures is.Valid()
+  {
+    var res := Utils.ReadFixedLengthFromStreamOrFail(is, 1);
+    match res {
+      case Success(contentType) =>
+        if contentType[0] == 0x01 {
+          return Success(NonFramed);
+        } else if contentType[0] == 0x02 {
+          return Success(Framed);
+        } else {
+          return Failure("Deserialization Error: Content type not supported.");
+        }
+      case Failure(e) => return Failure(e);
+    }
+  }
+
+  method DeserializeReserved(is: Streams.StringReader) returns (ret: Result<T_Reserved>)
+    requires is.Valid()
+    modifies is
+    ensures is.Valid()
+  {
+    var res := Utils.ReadFixedLengthFromStreamOrFail(is, 4);
+    match res {
+      case Success(reserved) =>
+        if reserved[0] == reserved[1] == reserved[2] == reserved[3] == 0 {
+          return Success(reserved[..]);
+        } else {
+          return Failure("Deserialization Error: Reserved fields must be 0.");
+        }
+      case Failure(e) => return Failure(e);
+    }
+  }
+
+  method DeserializeIVLength(is: Streams.StringReader, algSuiteId: AlgorithmSuite.ID) returns (ret: Result<uint8>)
+    requires is.Valid()
+    requires algSuiteId in AlgorithmSuite.Suite.Keys
+    ensures is.Valid()
+    modifies is
+    ensures match ret
+      case Success(ivLength) => ValidIVLength(ivLength, algSuiteId)
+      case Failure(_)       => true
+  {
+    var res := Utils.ReadFixedLengthFromStreamOrFail(is, 1);
+    match res {
+      case Success(ivLength) =>
+        if ivLength[0] == AlgorithmSuite.Suite[algSuiteId].params.ivLen {
+          return Success(ivLength[0]);
+        } else {
+          return Failure("Deserialization Error: Incorrect IV length.");
+        }
+      case Failure(e) => return Failure(e);
+    }
+  }
+
+  method DeserializeFrameLength(is: Streams.StringReader, contentType: T_ContentType) returns (ret: Result<uint32>)
+    requires is.Valid()
+    modifies is
+    ensures is.Valid()
+    ensures match ret
+      case Success(frameLength) => ValidFrameLength(frameLength, contentType)
+      case Failure(_) => true
+  {
+    var res := Utils.ReadFixedLengthFromStreamOrFail(is, 4);
+    match res {
+      case Success(frameLength) =>
+        if contentType.NonFramed? && ArrayToUInt32(frameLength) == 0 {
+          return Success(ArrayToUInt32(frameLength));
+        } else {
+          return Failure("Deserialization Error: Frame length must be 0 when content type is non-framed.");
+        }
+      case Failure(e) => return Failure(e);
+    }
+  }
+
+  /**
+  * Reads raw header data from the input stream and populates the header with all of the information about the
+  * message.
+  */
+  method DeserializeHeaderBody(is: Streams.StringReader) returns (ret: Result<HeaderBody>)
+    requires is.Valid()
+    modifies is
+    ensures is.Valid()
+    ensures match ret
+      case Success(hb) =>
+        && ValidHeaderBody(hb)
+      case Failure(_) => true
+  {
+    Assume(false);
+    reveal ValidHeaderBody();
+    var version: T_Version;
     {
-        ret := readFixedLengthFromStreamOrFail(is, n);
+      var res := DeserializeVersion(is);
+      match res {
+        case Success(version_) => version := version_;
+        case Failure(e)       => return Failure(e);
+      }
     }
 
-    // TODO: Probably this should be factored out into EncCtx at some point
-    method deserializeAAD(is: StringReader) returns (ret: Result<T_AAD>)
-        requires is.Valid()
-        modifies is
-        ensures
-            match ret
-                case Success(aad) =>
-                    && ValidAAD(aad)
-                case Failure(_) => true
-        ensures is.Valid()
+    var typ: T_Type;
     {
-        reveal ValidAAD();
-        var kvPairsLength: uint16;
-        {
-            var res := deserializeUnrestricted(is, 2);
-            match res {
-                case Success(bytes) => kvPairsLength := ArrayToUInt16(bytes);
-                case Failure(e) => return Failure(e);
-            }
-        }
-        if kvPairsLength == 0 {
-            return Success(EmptyAAD);
-        }
-        var totalBytesRead := 0;
-
-        var kvPairsCount: uint16;
-        {
-            var res := deserializeUnrestricted(is, 2);
-            match res {
-                case Success(bytes) =>
-                    kvPairsCount := ArrayToUInt16(bytes);
-                    totalBytesRead := totalBytesRead + bytes.Length;
-                    if kvPairsLength > 0 && kvPairsCount == 0 {
-                        return Failure("Deserialization Error: Key value pairs count is 0.");
-                    }
-                    assert kvPairsLength > 0 ==> kvPairsCount > 0;
-                case Failure(e) => return Failure(e);
-            }
-        }
-
-        // TODO: declare this array, make kvPairs a ghost, maintain invariant that sequence is a prefix of the array:
-        // var kvPairsArray: array<(seq<uint8>, seq<uint8>)> := new [kvPairsCount];
-        var kvPairs: seq<(seq<uint8>, seq<uint8>)> := [];
-        assert kvPairsCount > 0;
-
-        var i := 0;
-        while i < kvPairsCount
-            invariant is.Valid()
-            invariant |kvPairs| == i as int
-            invariant i <= kvPairsCount
-            invariant InBoundsKVPairsUpTo(kvPairs, i as nat)
-            invariant SortedKVPairsUpTo(kvPairs, i as nat)
-            invariant forall j :: 0 <= j < i ==> ValidUTF8Seq(kvPairs[j].0)
-            invariant forall j :: 0 <= j < i ==> ValidUTF8Seq(kvPairs[j].1)
-        {
-            var keyLength: uint16;
-            {
-                var res := deserializeUnrestricted(is, 2);
-                match res {
-                    case Success(bytes) =>
-                        keyLength := ArrayToUInt16(bytes);
-                        totalBytesRead := totalBytesRead + bytes.Length;
-                    case Failure(e) => return Failure(e);
-                }
-            }
-
-            var key: seq<uint8>;
-            {
-                var res := deserializeUTF8(is, keyLength as nat);
-                match res {
-                    case Success(bytes) =>
-                        ValidUTF8ArraySeq(bytes);
-                        key := bytes[..];
-                        totalBytesRead := totalBytesRead + bytes.Length;
-                    case Failure(e) => return Failure(e);
-                }
-            }
-            assert |key| < UINT16_LIMIT;
-            assert ValidUTF8Seq(key);
-
-            var valueLength: uint16;
-            {
-                var res := deserializeUnrestricted(is, 2);
-                match res {
-                    case Success(bytes) =>
-                        valueLength := ArrayToUInt16(bytes);
-                        totalBytesRead := totalBytesRead + bytes.Length;
-                    case Failure(e) => return Failure(e);
-                }
-            }
-
-            var value: seq<uint8>;
-            {
-                var res := deserializeUTF8(is, valueLength as nat);
-                match res {
-                    case Success(bytes) =>
-                        ValidUTF8ArraySeq(bytes);
-                        value := bytes[..];
-                        totalBytesRead := totalBytesRead + bytes.Length;
-                    case Failure(e) => return Failure(e);
-                }
-            }
-            assert |value| < UINT16_LIMIT;
-            assert ValidUTF8Seq(value);
-
-            // check for sortedness by key
-            if i != 0 && !LexCmpSeqs(kvPairs[i-1].0, key, ltByte) {
-                return Failure("Deserialization Error: Key-value pairs must be sorted by key.");
-            }
-            kvPairs := kvPairs + [(key, value)];
-            assert SortedKVPairsUpTo(kvPairs, (i+1) as nat);
-            i := i + 1;
-        }
-        if (kvPairsLength as nat) != totalBytesRead {
-            return Failure("Deserialization Error: Bytes actually read differs from bytes supposed to be read.");
-        }
-        return Success(AAD(kvPairs));
+      var res := DeserializeType(is);
+      match res {
+        case Success(typ_) => typ := typ_;
+        case Failure(e)   => return Failure(e);
+      }
     }
 
-    // TODO: Probably this should be factored out into EDK at some point
-    method deserializeEncryptedDataKeys(is: StringReader, ghost aad: T_AAD) returns (ret: Result<T_EncryptedDataKeys>)
-        requires is.Valid()
-        modifies is
-        ensures
-            match ret
-                case Success(edks) =>
-                    && ValidEncryptedDataKeys(edks)
-                case Failure(_)   => true
-        ensures is.Valid()
+    var algorithmSuiteID: AlgorithmSuite.ID;
     {
-        reveal ValidEncryptedDataKeys();
-        var edkCount: uint16;
-        var res := deserializeUnrestricted(is, 2);
-        match res {
-            case Success(bytes) => edkCount := ArrayToUInt16(bytes);
-            case Failure(e)    => return Failure(e);
-        }
-
-        if edkCount == 0 {
-            return Failure("Deserialization Error: Encrypted data key count must be > 0.");
-        }
-
-        var edkEntries: seq<EDKEntry> := [];
-        var i := 0;
-        while i < edkCount
-            invariant is.Valid()
-            invariant i <= edkCount
-            invariant InBoundsEncryptedDataKeys(edkEntries)
-        {
-            // Key provider ID
-            var keyProviderIDLength: uint16;
-            res := deserializeUnrestricted(is, 2);
-            match res {
-                case Success(bytes) => keyProviderIDLength := ArrayToUInt16(bytes);
-                case Failure(e)    => return Failure(e);
-            }
-
-            var keyProviderID: string;
-            res := deserializeUTF8(is, keyProviderIDLength as nat);
-            match res {
-                case Success(bytes) => keyProviderID := ByteSeqToString(bytes[..]);
-                case Failure(e)    => return Failure(e);
-            }
-
-            // Key provider info
-            var keyProviderInfoLength: uint16;
-            res := deserializeUnrestricted(is, 2);
-            match res {
-                case Success(bytes) => keyProviderInfoLength := ArrayToUInt16(bytes);
-                case Failure(e)    => return Failure(e);
-            }
-
-            var keyProviderInfo: seq<uint8>;
-            res := deserializeUnrestricted(is, keyProviderInfoLength as nat);
-            match res {
-                case Success(bytes) => keyProviderInfo := bytes[..];
-                case Failure(e)    => return Failure(e);
-            }
-
-            // Encrypted data key
-            var edkLength: uint16;
-            res := deserializeUnrestricted(is, 2);
-            match res {
-                case Success(bytes) => edkLength := ArrayToUInt16(bytes);
-                case Failure(e)    => return Failure(e);
-            }
-
-            var edk: seq<uint8>;
-            res := deserializeUnrestricted(is, edkLength as nat);
-            match res {
-                case Success(bytes) => edk := bytes[..];
-                case Failure(e)    => return Failure(e);
-            }
-
-            edkEntries := edkEntries + [Materials.EncryptedDataKey(keyProviderID, keyProviderInfo, edk)];
-            i := i + 1;
-        }
-
-        var edks := EncryptedDataKeys(edkEntries);
-        return Success(edks);
+      var res := DeserializeAlgorithmSuiteID(is);
+      match res {
+        case Success(algorithmSuiteID_) => algorithmSuiteID := algorithmSuiteID_;
+        case Failure(e)                => return Failure(e);
+      }
     }
 
-    method deserializeContentType(is: StringReader) returns (ret: Result<T_ContentType>)
-        requires is.Valid()
-        modifies is
-        ensures is.Valid()
+    var messageID: T_MessageID;
     {
-        var res := readFixedLengthFromStreamOrFail(is, 1);
-        match res {
-            case Success(contentType) =>
-                if contentType[0] == 0x01 {
-                    return Success(NonFramed);
-                } else if contentType[0] == 0x02 {
-                    return Success(Framed);
-                } else {
-                    return Failure("Deserialization Error: Content type not supported.");
-                }
-            case Failure(e) => return Failure(e);
-        }
+      var res := DeserializeMsgID(is);
+      match res {
+        case Success(messageID_) => messageID := messageID_;
+        case Failure(e)    => return Failure(e);
+      }
     }
 
-    method deserializeReserved(is: StringReader) returns (ret: Result<T_Reserved>)
-        requires is.Valid()
-        modifies is
-        ensures is.Valid()
+    // AAD deserialization:
+    var aad: T_AAD;
     {
-        var res := readFixedLengthFromStreamOrFail(is, 4);
-        match res {
-            case Success(reserved) =>
-                if reserved[0] == reserved[1] == reserved[2] == reserved[3] == 0 {
-                    return Success(reserved[..]);
-                } else {
-                    return Failure("Deserialization Error: Reserved fields must be 0.");
-                }
-            case Failure(e) => return Failure(e);
-        }
+      var res := DeserializeAAD(is);
+      match res {
+        case Success(aad_) => aad := aad_;
+        case Failure(e)   => return Failure(e);
+      }
     }
 
-    method deserializeIVLength(is: StringReader, algSuiteId: AlgorithmSuite.ID) returns (ret: Result<uint8>)
-        requires is.Valid()
-        requires algSuiteId in AlgorithmSuite.Suite.Keys
-        modifies is
-        ensures
-            match ret
-                case Success(ivLength) => ValidIVLength(ivLength, algSuiteId)
-                case Failure(_)       => true
-        ensures is.Valid()
+    // EDK deserialization:
+    var encryptedDataKeys: T_EncryptedDataKeys;
     {
-        var res := readFixedLengthFromStreamOrFail(is, 1);
-        match res {
-            case Success(ivLength) =>
-                if ivLength[0] == AlgorithmSuite.Suite[algSuiteId].params.ivLen {
-                    return Success(ivLength[0]);
-                } else {
-                    return Failure("Deserialization Error: Incorrect IV length.");
-                }
-            case Failure(e) => return Failure(e);
-        }
+      var res := DeserializeEncryptedDataKeys(is, aad);
+      match res {
+        case Success(encryptedDataKeys_) => encryptedDataKeys := encryptedDataKeys_;
+        case Failure(e)   => return Failure(e);
+      }
     }
 
-    method deserializeFrameLength(is: StringReader, contentType: T_ContentType) returns (ret: Result<uint32>)
-        requires is.Valid()
-        modifies is
-        ensures
-            match ret
-                case Success(frameLength) => ValidFrameLength(frameLength, contentType)
-                case Failure(_) => true
-        ensures is.Valid()
+    var contentType: T_ContentType;
     {
-        var res := readFixedLengthFromStreamOrFail(is, 4);
-        match res {
-            case Success(frameLength) =>
-                if contentType.NonFramed? && ArrayToUInt32(frameLength) == 0 {
-                    return Success(ArrayToUInt32(frameLength));
-                } else {
-                    return Failure("Deserialization Error: Frame length must be 0 when content type is non-framed.");
-                }
-            case Failure(e) => return Failure(e);
-        }
+      var res := DeserializeContentType(is);
+      match res {
+        case Success(contentType_) => contentType := contentType_;
+        case Failure(e)           => return Failure(e);
+      }
     }
-    /**
-    * Reads raw header data from the input stream and populates the header with all of the information about the
-    * message.
-    */
-    method headerBody(is: StringReader) returns (ret: Result<HeaderBody>)
-        requires is.Valid()
-        modifies is
-        ensures is.Valid()
-        ensures
-            match ret
-                case Success(hb) =>
-                    && ValidHeaderBody(hb)
-                case Failure(_) => true
+
+    var reserved: T_Reserved;
     {
-        Assume(false);
-        reveal ValidHeaderBody();
-        var version: T_Version;
-        {
-            var res := deserializeVersion(is);
-            match res {
-                case Success(version_) => version := version_;
-                case Failure(e)       => return Failure(e);
-            }
-        }
-
-        var typ: T_Type;
-        {
-            var res := deserializeType(is);
-            match res {
-                case Success(typ_) => typ := typ_;
-                case Failure(e)   => return Failure(e);
-            }
-        }
-
-        var algorithmSuiteID: AlgorithmSuite.ID;
-        {
-            var res := deserializeAlgorithmSuiteID(is);
-            match res {
-                case Success(algorithmSuiteID_) => algorithmSuiteID := algorithmSuiteID_;
-                case Failure(e)                => return Failure(e);
-            }
-        }
-
-        var messageID: T_MessageID;
-        {
-            var res := deserializeMsgID(is);
-            match res {
-                case Success(messageID_) => messageID := messageID_;
-                case Failure(e)    => return Failure(e);
-            }
-        }
-
-        // AAD deserialization:
-        var aad: T_AAD;
-        {
-            var res := deserializeAAD(is);
-            match res {
-                case Success(aad_) => aad := aad_;
-                case Failure(e)   => return Failure(e);
-            }
-        }
-
-        // EDK deserialization:
-        var encryptedDataKeys: T_EncryptedDataKeys;
-        {
-            var res := deserializeEncryptedDataKeys(is, aad);
-            match res {
-                case Success(encryptedDataKeys_) => encryptedDataKeys := encryptedDataKeys_;
-                case Failure(e)   => return Failure(e);
-            }
-        }
-
-        var contentType: T_ContentType;
-        {
-            var res := deserializeContentType(is);
-            match res {
-                case Success(contentType_) => contentType := contentType_;
-                case Failure(e)           => return Failure(e);
-            }
-        }
-
-        var reserved: T_Reserved;
-        {
-            var res := deserializeReserved(is);
-            match res {
-                case Success(reserved_) => reserved := reserved_;
-                case Failure(e)    => return Failure(e);
-            }
-        }
-
-        var ivLength: uint8;
-        {
-            var res := deserializeIVLength(is, algorithmSuiteID);
-            match res {
-                case Success(ivLength_) => ivLength := ivLength_;
-                case Failure(e)    => return Failure(e);
-            }
-        }
-
-        var frameLength: uint32;
-        {
-            var res := deserializeFrameLength(is, contentType);
-            match res {
-                case Success(frameLength_) => frameLength := frameLength_;
-                case Failure(e) => return Failure(e);
-            }
-        }
-        var hb := HeaderBody(
-                    version,
-                    typ,
-                    algorithmSuiteID,
-                    messageID,
-                    aad,
-                    encryptedDataKeys,
-                    contentType,
-                    reserved,
-                    ivLength,
-                    frameLength);
-        assert ValidHeaderBody(hb);
-        ret := Success(hb);
+      var res := DeserializeReserved(is);
+      match res {
+        case Success(reserved_) => reserved := reserved_;
+        case Failure(e)    => return Failure(e);
+      }
     }
 
-    method deserializeAuthenticationTag(is: StringReader, tagLength: nat, ghost iv: array<uint8>) returns (ret: Result<array<uint8>>)
-        requires is.Valid()
-        modifies is
-        ensures
-            match ret
-                case Success(authenticationTag) => ValidAuthenticationTag(authenticationTag, tagLength, iv)
-                case Failure(_) => true
-        ensures is.Valid()
+    var ivLength: uint8;
     {
-        ret := readFixedLengthFromStreamOrFail(is, tagLength);
+      var res := DeserializeIVLength(is, algorithmSuiteID);
+      match res {
+        case Success(ivLength_) => ivLength := ivLength_;
+        case Failure(e)    => return Failure(e);
+      }
     }
 
-    method headerAuthentication(is: StringReader, body: HeaderBody) returns (ret: Result<HeaderAuthentication>)
-        requires is.Valid()
-        requires ValidHeaderBody(body)
-        requires body.algorithmSuiteID in AlgorithmSuite.Suite.Keys
-        modifies is
-        ensures is.Valid()
-        ensures
-            match ret
-                case Success(headerAuthentication) =>
-                    && ValidHeaderAuthentication(headerAuthentication, body.algorithmSuiteID)
-                    && ValidHeaderBody(body)
-                case Failure(_) => true
+    var frameLength: uint32;
     {
-        var iv: array<uint8>;
-        {
-            var res := deserializeUnrestricted(is, body.ivLength as nat);
-            match res {
-                case Success(bytes) => iv := bytes;
-                case Failure(e)    => return Failure(e);
-            }
-        }
-
-        var authenticationTag: array<uint8>;
-        {
-            var res := deserializeAuthenticationTag(is, AlgorithmSuite.Suite[body.algorithmSuiteID].params.tagLen as nat, iv);
-            match res {
-                case Success(bytes) => authenticationTag := bytes;
-                case Failure(e)    => return Failure(e);
-            }
-        }
-        ret := Success(HeaderAuthentication(iv, authenticationTag));
+      var res := DeserializeFrameLength(is, contentType);
+      match res {
+        case Success(frameLength_) => frameLength := frameLength_;
+        case Failure(e) => return Failure(e);
+      }
     }
+    var hb := HeaderBody(
+      version,
+      typ,
+      algorithmSuiteID,
+      messageID,
+      aad,
+      encryptedDataKeys,
+      contentType,
+      reserved,
+      ivLength,
+      frameLength);
+    assert ValidHeaderBody(hb);
+    ret := Success(hb);
+  }
+
+  method DeserializeAuthenticationTag(is: Streams.StringReader, tagLength: nat, ghost iv: array<uint8>) returns (ret: Result<array<uint8>>)
+    requires is.Valid()
+    modifies is
+    ensures is.Valid()
+    ensures match ret
+      case Success(authenticationTag) => ValidAuthenticationTag(authenticationTag, tagLength, iv)
+      case Failure(_) => true
+  {
+    ret := Utils.ReadFixedLengthFromStreamOrFail(is, tagLength);
+  }
+
+  method DeserializeAuthenticationHeader(is: Streams.StringReader, body: HeaderBody) returns (ret: Result<HeaderAuthentication>)
+    requires is.Valid()
+    requires ValidHeaderBody(body)
+    requires body.algorithmSuiteID in AlgorithmSuite.Suite.Keys
+    modifies is
+    ensures is.Valid()
+    ensures match ret
+      case Success(headerAuthentication) =>
+        && ValidHeaderAuthentication(headerAuthentication, body.algorithmSuiteID)
+        && ValidHeaderBody(body)
+      case Failure(_) => true
+  {
+    var iv: array<uint8>;
+    {
+      var res := DeserializeUnrestricted(is, body.ivLength as nat);
+      match res {
+        case Success(bytes) => iv := bytes;
+        case Failure(e)    => return Failure(e);
+      }
+    }
+
+    var authenticationTag: array<uint8>;
+    {
+      var res := DeserializeAuthenticationTag(is, AlgorithmSuite.Suite[body.algorithmSuiteID].params.tagLen as nat, iv);
+      match res {
+        case Success(bytes) => authenticationTag := bytes;
+        case Failure(e)    => return Failure(e);
+      }
+    }
+    ret := Success(HeaderAuthentication(iv, authenticationTag));
+  }
 }
