src/SDK/MessageHeader/Utils.dfy
@@ -4,118 +4,114 @@ include "../../StandardLibrary/StandardLibrary.dfy"
 include "../../Util/UTF8.dfy"
 
 module MessageHeader.Utils {
-    import AlgorithmSuite
-    import opened Streams
-    import opened StandardLibrary
-    import opened UInt = StandardLibrary.UInt
-    import opened UTF8
-    /*
-     * Utils
-     */
-    method readFixedLengthFromStreamOrFail(is: StringReader, n: nat) returns (ret: Result<array<uint8>>)
-        requires is.Valid()
-        modifies is
-        ensures
-            match ret
-                case Success(bytes) =>
-                    && n == bytes.Length
-                    && fresh(bytes)
-                case Failure(_)    => true
-        ensures is.Valid()
-    {
-        var bytes := new uint8[n];
-        var out := is.Read(bytes, 0, n);
-        match out {
-            case Success(bytesRead) =>
-                if bytesRead != n {
-                    return Failure("IO Error: Not enough bytes left on stream.");
-                } else {
-                    return Success(bytes);
-                }
-            case Failure(e) => return Failure(e);
+  import AlgorithmSuite
+  import Streams
+  import opened StandardLibrary
+  import opened UInt = StandardLibrary.UInt
+  /*
+   * Utils
+   */
+  method ReadFixedLengthFromStreamOrFail(is: Streams.StringReader, n: nat) returns (ret: Result<array<uint8>>)
+    requires is.Valid()
+    modifies is
+    ensures is.Valid()
+    ensures match ret
+      case Success(bytes) =>
+        && n == bytes.Length
+        && fresh(bytes)
+      case Failure(_) => true
+  {
+    var bytes := new uint8[n];
+    var out := is.Read(bytes, 0, n);
+    match out {
+      case Success(bytesRead) =>
+        if bytesRead != n {
+          return Failure("IO Error: Not enough bytes left on stream.");
+        } else {
+          return Success(bytes);
         }
+      case Failure(e) => return Failure(e);
     }
-    /*
-    // This is like StringWriter.WriteSimple
-    // TODO: this is broken somehow
-    method WriteFixedLengthToStreamOrFail(os: StringWriter, bytes: array<uint8>) returns (ret: Result<nat>)
-      requires os.Valid()
-      requires bytes !in os.Repr
-      modifies os.Repr
-      ensures old(os.Repr) == os.Repr
-      ensures bytes !in os.Repr
-      ensures os.Valid()
-      ensures
-        match ret
-          case Success(len_written) =>
-            && len_written == bytes.Length
-            && os.pos == old(os.pos) + len_written
-            && old(os.pos + len_written <= os.data.Length)
-            && os.data[..] == old(os.data[..os.pos]) + bytes[..] + old(os.data[os.pos + len_written..])
-          case Failure(e) => true
-    {
-        ghost var oldPos := os.pos;
-        ghost var oldData := os.data;
-        var oldCap := os.capacity();
-        ret := os.Write(bytes, 0, bytes.Length);
-        match ret {
-            case Success(len) =>
-                if oldCap >= bytes.Length > 0 {
-                //if len == bytes.Length {
-                   // assert len == bytes.Length;
-                    assert oldPos + len <= oldData.Length;
+  }
+  /*
+  // This is like StringWriter.WriteSimple
+  // TODO: this is broken somehow
+  method WriteFixedLengthToStreamOrFail(os: Streams.StringWriter, bytes: array<uint8>) returns (ret: Result<nat>)
+    requires os.Valid()
+    requires bytes !in os.Repr
+    modifies os.Repr
+    ensures old(os.Repr) == os.Repr
+    ensures bytes !in os.Repr
+    ensures os.Valid()
+    ensures match ret
+      case Success(len_written) =>
+        && len_written == bytes.Length
+        && os.pos == old(os.pos) + len_written
+        && old(os.pos + len_written <= os.data.Length)
+        && os.data[..] == old(os.data[..os.pos]) + bytes[..] + old(os.data[os.pos + len_written..])
+      case Failure(e) => true
+  {
+    ghost var oldPos := os.pos;
+    ghost var oldData := os.data;
+    var oldCap := os.capacity();
+    ret := os.Write(bytes, 0, bytes.Length);
+    match ret {
+      case Success(len) =>
+        if oldCap >= bytes.Length > 0 {
+        //if len == bytes.Length {
+          // assert len == bytes.Length;
+          assert oldPos + len <= oldData.Length;
 
-                    assert os.data[..oldPos] == oldData[..oldPos];
-                    assert os.data[oldPos..oldPos+len] == bytes[..];
-                    assert os.data[oldPos+len..] == oldData[oldPos + len..];
+          assert os.data[..oldPos] == oldData[..oldPos];
+          assert os.data[oldPos..oldPos+len] == bytes[..];
+          assert os.data[oldPos+len..] == oldData[oldPos + len..];
 
-                    assert os.data[..] == oldData[..oldPos] + bytes[..] + oldData[oldPos + len..];
-                    assert os.pos == oldPos + len;
-                    return Success(len);
-                } else {
-                    return Failure("Serialization Error: Reached end of stream.");
-                }
-            case Failure(e)  => return ret;
+          assert os.data[..] == oldData[..oldPos] + bytes[..] + oldData[oldPos + len..];
+          assert os.pos == oldPos + len;
+          return Success(len);
+        } else {
+          return Failure("Serialization Error: Reached end of stream.");
         }
+      case Failure(e)  => return ret;
     }
-    */
-    /*
-    // This is like StringWriter.WriteSingleByteSimple
-    method WriteSingleByteToStreamOrFail(os: StringWriter, byte: uint8) returns (ret: Result<nat>)
-      requires os.Valid()
-      modifies os.Repr
-      ensures old(os.Repr) == os.Repr
-      ensures os.Valid()
-      ensures
-        match ret
-          case Success(len_written) =>
-            && len_written == 1
-            && old(os.pos + len_written <= os.data.Length)
-            && os.data[..] == old(os.data[..os.pos]) + [byte] + old(os.data[os.pos + len_written..])
-            && os.pos == old(os.pos) + len_written
-          case Failure(e) => true
-    {
-        ret := os.WriteSingleByte(byte);
-        match ret {
-            case Success(len) =>
-                if len == 1 {
-                    return Success(len);
-                } else {
-                    return Failure("Serialization Error: Reached end of stream.");
-                }
-            case Failure(e)  => return ret;
+  }
+  */
+  /*
+  // This is like StringWriter.WriteSingleByteSimple
+  method WriteSingleByteToStreamOrFail(os: Streams.StringWriter, byte: uint8) returns (ret: Result<nat>)
+    requires os.Valid()
+    modifies os.Repr
+    ensures old(os.Repr) == os.Repr
+    ensures os.Valid()
+    ensures match ret
+      case Success(len_written) =>
+        && len_written == 1
+        && old(os.pos + len_written <= os.data.Length)
+        && os.data[..] == old(os.data[..os.pos]) + [byte] + old(os.data[os.pos + len_written..])
+        && os.pos == old(os.pos) + len_written
+      case Failure(e) => true
+  {
+    ret := os.WriteSingleByte(byte);
+    match ret {
+      case Success(len) =>
+        if len == 1 {
+          return Success(len);
+        } else {
+          return Failure("Serialization Error: Reached end of stream.");
         }
+      case Failure(e)  => return ret;
     }
-    */
+  }
+  */
 
-    predicate SortedKVPairsUpTo(a: seq<(seq<uint8>, seq<uint8>)>, n: nat)
-        requires n <= |a|
-    {
-        forall j :: 0 < j < n ==> LexCmpSeqs(a[j-1].0, a[j].0, ltByte)
-    }
+  predicate SortedKVPairsUpTo(a: seq<(seq<uint8>, seq<uint8>)>, n: nat)
+    requires n <= |a|
+  {
+    forall j :: 0 < j < n ==> LexCmpSeqs(a[j-1].0, a[j].0, UInt8Less)
+  }
 
-    predicate SortedKVPairs(a: seq<(seq<uint8>, seq<uint8>)>)
-    {
-        SortedKVPairsUpTo(a, |a|)
-    }
+  predicate SortedKVPairs(a: seq<(seq<uint8>, seq<uint8>)>)
+  {
+    SortedKVPairsUpTo(a, |a|)
+  }
 }
